Remove common base for semantic type and value
They are unnecessary. Actually, I'm more questioning now whether the
distinction of the names is necessary. Semantic formalizations until now
does not use it anymore! The equality comparison in the automation is
all syntactical. Maybe one day I will remove the semantic equality
mechanism (i.e. the name locale in the virtual datatype) meaning we
actually don't need the virtual datatype to formalize the type and value
semantics, but maybe just locales of projection and injection pair!

Phi_Semantics/PhiSem_Aggregate.thy
@@ -1,5 +1,5 @@
 theory PhiSem_Aggregate
-  imports Phi_System.PhiSem_Formalization_Tools
+  imports PhiSem_Aggregate_Base
 begin
 
 section \<open>Semantics\<close>
@@ -56,37 +56,20 @@ hide_fact aggregate_val_ax
 subsection \<open>Semantics\<close>
 
 debt_axiomatization
-        valid_idx_step :: \<open>TY \<Rightarrow> nat \<Rightarrow> bool\<close>
-    and idx_step_type  :: \<open>nat \<Rightarrow> TY \<Rightarrow> TY\<close>
-    and idx_step_value :: \<open>nat \<Rightarrow> VAL \<Rightarrow> VAL\<close>
-    and idx_step_mod_value :: \<open>nat \<Rightarrow> (VAL \<Rightarrow> VAL) \<Rightarrow> VAL \<Rightarrow> VAL\<close>
-    and type_measure :: \<open>TY \<Rightarrow> nat\<close>
-  where WT_tup[simp]: \<open>Well_Type (tup ts)  = { V_tup.mk vs       |vs. list_all2 (\<lambda> t v. v \<in> Well_Type t) ts vs }\<close>
+        WT_tup[simp]: \<open>Well_Type (tup ts)  = { V_tup.mk vs       |vs. list_all2 (\<lambda> t v. v \<in> Well_Type t) ts vs }\<close>
   and   WT_arr[simp]: \<open>Well_Type (array n t) = { V_array.mk (t,vs) |vs. length vs = n \<and> list_all (\<lambda>v. v \<in> Well_Type t) vs \<and> Valid_Type t }\<close>
   and   zero_tup[simp]: \<open>Zero (tup Ts)     = map_option V_tup.mk (those (map Zero Ts))\<close>
   and   zero_arr[simp]: \<open>Zero (array N T)  = map_option (\<lambda>z. V_array.mk (T, replicate N z)) (Zero T)\<close>
   and   V_tup_sep_disj[simp]: \<open>V_tup.mk l1 ## V_tup.mk l2\<close>
   and   V_tup_mult    : \<open>V_tup.mk l1 * V_tup.mk l2 = V_tup.mk (l2 @ l1)\<close>
-  and   idx_step_type_measure: \<open>valid_idx_step T i
-                            \<Longrightarrow> type_measure (idx_step_type i T) < type_measure T\<close>
+(*  and   idx_step_type_measure: \<open>valid_idx_step T i
+                            \<Longrightarrow> type_measure (idx_step_type i T) < type_measure T\<close>*)
   and   idx_step_type_tup  : \<open>i < length tys \<Longrightarrow> idx_step_type i (tup tys) = tys!i \<close>
   and   idx_step_type_arr  : \<open>i \<le> N \<Longrightarrow> idx_step_type i (array N T) = T\<close>
   and   valid_idx_step_tup : \<open>valid_idx_step (tup tys) i \<longleftrightarrow> i < length tys\<close>
   and   valid_idx_step_arr : \<open>valid_idx_step (array N T) i \<longleftrightarrow> i < N\<close>
-  and   idx_step_value_welltyp: \<open>valid_idx_step T i
-                             \<Longrightarrow> v \<in> Well_Type T
-                             \<Longrightarrow> idx_step_value i v \<in> Well_Type (idx_step_type i T)\<close>
   and   idx_step_value_tup : \<open>idx_step_value i (V_tup.mk vs)   = vs!i\<close>
   and   idx_step_value_arr : \<open>idx_step_value i (V_array.mk (T,vs)) = vs!i\<close>
-  and   idx_step_mod_value : \<open>valid_idx_step T i
-                          \<Longrightarrow> valid_idx_step T j
-                          \<Longrightarrow> v \<in> Well_Type T
-                          \<Longrightarrow> idx_step_value i (idx_step_mod_value j f v) =
-                                (if i = j then f (idx_step_value j v) else idx_step_value i v) \<close>
-  and   idx_step_mod_value_welltyp: \<open>valid_idx_step T i
-                                 \<Longrightarrow> v \<in> Well_Type T
-                                 \<Longrightarrow> f (idx_step_value i v) \<in> Well_Type (idx_step_type i T)
-                                 \<Longrightarrow> idx_step_mod_value i f v \<in> Well_Type T\<close>
   and   idx_step_mod_value_tup : \<open>idx_step_mod_value i f (V_tup.mk vs) = V_tup.mk (vs[i := f (vs!i)])\<close>
   and   idx_step_mod_value_arr : \<open>idx_step_mod_value i f (V_array.mk (T,vs)) = V_array.mk (T,vs[i := f (vs!i)])\<close>
 
@@ -95,41 +78,8 @@ lemma V_tup_mult_cons:
   \<open>NO_MATCH vs ([]::VAL list) \<Longrightarrow> V_tup.mk (v#vs) = V_tup.mk vs * V_tup.mk [v]\<close>
   using V_tup_mult by simp
 
-abbreviation \<open>index_value \<equiv> fold idx_step_value\<close>
-abbreviation \<open>index_type  \<equiv> fold idx_step_type\<close>
-abbreviation \<open>index_mod_value \<equiv> foldr idx_step_mod_value\<close>
 
-primrec valid_index :: \<open>TY \<Rightarrow> nat list \<Rightarrow> bool\<close>
-  where \<open>valid_index T [] \<longleftrightarrow> True\<close>
-      | \<open>valid_index T (i#idx) \<longleftrightarrow> valid_idx_step T i \<and> valid_index (idx_step_type i T) idx\<close>
 
-lemma valid_index_tail[simp]:
-  \<open>valid_index T (idx@[i]) \<longleftrightarrow> valid_index T idx \<and> valid_idx_step (index_type idx T) i\<close>
-  by (induct idx arbitrary: T; simp)
-
-lemma index_type_measure:
-  \<open>valid_index T idx \<Longrightarrow> idx \<noteq> [] \<Longrightarrow> type_measure (index_type idx T) < type_measure T\<close>
-  apply (induct idx arbitrary: T; simp)
-  by (metis dual_order.strict_trans fold_simps(1) idx_step_type_measure)
-
-lemma valid_index_cat: \<open>valid_index T (a@b) \<Longrightarrow> valid_index T a \<and> valid_index (index_type a T) b\<close>
-  by (induct a arbitrary: T; simp)
-
-lemma valid_index_cons: \<open>valid_index T [i] \<longleftrightarrow> valid_idx_step T i\<close> by simp
-
-lemma index_value_welltyp:
-  \<open>valid_index T idx \<Longrightarrow> v \<in> Well_Type T \<Longrightarrow> index_value idx v \<in> Well_Type (index_type idx T)\<close>
-  apply (induct idx arbitrary: v T; simp)
-  using idx_step_value_welltyp
-  by blast
-
-lemma index_mod_value_welltyp:
-   \<open>valid_index T idx
-\<Longrightarrow> v \<in> Well_Type T
-\<Longrightarrow> f (index_value idx v) \<in> Well_Type (index_type idx T)
-\<Longrightarrow> index_mod_value idx f v \<in> Well_Type T\<close>
-  apply (induct idx arbitrary: T v; simp)
-  using idx_step_mod_value_welltyp idx_step_value_welltyp by blast
 
 
 
@@ -143,11 +93,6 @@ lemma index_offset_tail[simp]:
   \<open>index_offset T (idx@[i]) = index_offset T idx + idx_step_offset (index_type idx T) i\<close>
   by (induct idx arbitrary: T; simp) *)
 
-lemma index_type_idem:
-  \<open>valid_index T idx \<Longrightarrow> index_type idx T = T \<longleftrightarrow> idx = []\<close>
-  apply (cases idx; simp; rule)
-  using index_type_measure
-  by (metis fold_simps(2) list.discI order_less_irrefl valid_index.simps(2))
 
 lemma list_all_replicate:
   \<open>list_all P (replicate n x) \<longleftrightarrow> n = 0 \<or> P x\<close>
@@ -179,48 +124,54 @@ lemma EmptyTuple_expn[\<phi>expns]:
 
 subsubsection \<open>Field\<close>
 
-definition \<phi>Field :: "(VAL, 'a) \<phi> \<Rightarrow> (VAL, 'a) \<phi>" ("\<clubsuit>")
-  where "\<phi>Field T x = { V_tup.mk [v] |v. v \<in> T x }"
+definition Tuple_Field :: "(VAL, 'a) \<phi> \<Rightarrow> (VAL, 'a) \<phi>"
+  where "Tuple_Field T x = { V_tup.mk [v] |v. v \<in> T x }"
 
-lemma \<phi>Field_expn[\<phi>expns]:
-  \<open>p \<in> (x \<Ztypecolon> \<phi>Field T) \<longleftrightarrow> (\<exists>v. p = V_tup.mk [v] \<and> v \<in> (x \<Ztypecolon> T))\<close>
-  unfolding \<phi>Field_def \<phi>Type_def by simp
+syntax "_\<phi>Tuple" :: \<open>tuple_args \<Rightarrow> logic\<close> ("\<lbrace> _ \<rbrace>")
 
-lemma \<phi>Field_inhabited[elim!,\<phi>inhabitance_rule]:
-  \<open>Inhabited (x \<Ztypecolon> \<clubsuit> T) \<Longrightarrow> (Inhabited (x \<Ztypecolon> T) \<Longrightarrow> C) \<Longrightarrow> C\<close>
+translations
+  "_\<phi>Tuple (_tuple_arg X)" \<rightleftharpoons> "CONST Tuple_Field X"
+  "_\<phi>Tuple (_tuple_args y z)" \<rightleftharpoons> "CONST \<phi>Prod (_\<phi>Tuple (_tuple_arg y)) (_\<phi>Tuple z)"
+
+lemma Tuple_Field_expn[\<phi>expns]:
+  \<open>p \<in> (x \<Ztypecolon> \<lbrace> T \<rbrace>) \<longleftrightarrow> (\<exists>v. p = V_tup.mk [v] \<and> v \<in> (x \<Ztypecolon> T))\<close>
+  unfolding Tuple_Field_def \<phi>Type_def by simp
+
+lemma Tuple_Field_inhabited[elim!,\<phi>inhabitance_rule]:
+  \<open>Inhabited (x \<Ztypecolon> \<lbrace> T \<rbrace>) \<Longrightarrow> (Inhabited (x \<Ztypecolon> T) \<Longrightarrow> C) \<Longrightarrow> C\<close>
   unfolding Inhabited_def by (simp add: \<phi>expns)
 
 lemma EmptyTuple_reduce[simp]:
-  \<open>(((),a) \<Ztypecolon> EmptyTuple \<^emph> \<clubsuit> T) = (a \<Ztypecolon> \<clubsuit> T)\<close>
-  \<open>((a,()) \<Ztypecolon> \<clubsuit> T \<^emph> EmptyTuple) = (a \<Ztypecolon> \<clubsuit> T)\<close>
+  \<open>(((),a) \<Ztypecolon> EmptyTuple \<^emph> \<lbrace> T \<rbrace>) = (a \<Ztypecolon> \<lbrace> T \<rbrace>)\<close>
+  \<open>((a,()) \<Ztypecolon> \<lbrace> T \<rbrace> \<^emph> EmptyTuple) = (a \<Ztypecolon> \<lbrace> T \<rbrace>)\<close>
   unfolding set_eq_iff
   apply (clarsimp; rule; clarsimp simp add: \<phi>expns V_tup_mult)
   apply (metis V_tup_mult V_tup_sep_disj append_Nil)
   apply (clarsimp; rule; clarsimp simp add: \<phi>expns V_tup_mult)
   by (metis V_tup_mult V_tup_sep_disj append_Cons append_Nil)
 
-lemma \<phi>Field_zero  [\<phi>reason 1000]:
-  \<open>\<phi>Zero ty T x \<Longrightarrow> \<phi>Zero (tup [ty]) (\<clubsuit> T) x \<close>
+lemma Tuple_Field_zero  [\<phi>reason 1000]:
+  \<open>\<phi>Zero ty T x \<Longrightarrow> \<phi>Zero (tup [ty]) \<lbrace> T \<rbrace> x \<close>
   unfolding \<phi>Zero_def by (clarsimp simp add: \<phi>expns)
 
-lemma \<phi>Field_zeros [\<phi>reason 1000]:
+lemma Tuple_Field_zeros [\<phi>reason 1000]:
   \<open>\<phi>Zero ty T x
     \<Longrightarrow> \<phi>Zero (tup tys) Ts xs
-    \<Longrightarrow> \<phi>Zero (tup (ty#tys)) (\<clubsuit> T \<^emph> Ts) (x,xs) \<close>
+    \<Longrightarrow> \<phi>Zero (tup (ty#tys)) (\<lbrace> T \<rbrace> \<^emph> Ts) (x,xs) \<close>
   unfolding \<phi>Zero_def
   apply (clarsimp simp add: \<phi>expns V_tup_mult_cons image_iff)
   using V_tup_sep_disj by blast
 
 
-lemma \<phi>Field_semty[\<phi>reason 1000]:
-  \<open>\<phi>SemType (x \<Ztypecolon> T) TY \<Longrightarrow> \<phi>SemType (x \<Ztypecolon> \<clubsuit> T) (tup [TY])\<close>
+lemma Tuple_Field_semty[\<phi>reason 1000]:
+  \<open>\<phi>SemType (x \<Ztypecolon> T) TY \<Longrightarrow> \<phi>SemType (x \<Ztypecolon> \<lbrace> T \<rbrace>) (tup [TY])\<close>
   unfolding \<phi>SemType_def subset_iff
   by (clarsimp simp add: \<phi>expns)
 
-lemma \<phi>Field_semtsy[\<phi>reason 1000]:
+lemma Tuple_Field_semtys[\<phi>reason 1000]:
   \<open> \<phi>SemType (x \<Ztypecolon> T) TY
 \<Longrightarrow> \<phi>SemType (xs \<Ztypecolon> Ts) (tup TYs)
-\<Longrightarrow> \<phi>SemType ((x,xs) \<Ztypecolon> (\<clubsuit> T \<^emph> Ts)) (tup (TY#TYs))\<close>
+\<Longrightarrow> \<phi>SemType ((x,xs) \<Ztypecolon> (\<lbrace> T \<rbrace> \<^emph> Ts)) (tup (TY#TYs))\<close>
   unfolding \<phi>SemType_def subset_iff
   apply (clarsimp simp add: \<phi>expns)
   by (metis V_tup_mult append.left_neutral append_Cons list.rel_inject(2))
@@ -292,6 +243,12 @@ definition \<phi>Index_getter :: \<open>nat list \<Rightarrow> (VAL,'a) \<phi> \
 definition \<phi>Index_mapper :: \<open>nat list \<Rightarrow> (VAL,'a) \<phi> \<Rightarrow> (VAL,'b) \<phi> \<Rightarrow> (('b \<Rightarrow> 'b) \<Rightarrow> 'a \<Rightarrow> 'a) \<Rightarrow> bool\<close>
   where \<open>\<phi>Index_mapper idx T U f \<longleftrightarrow> (\<forall>g g'. g \<in> (g' \<Ztypecolon> U \<Rrightarrow> U) \<longrightarrow> index_mod_value idx g \<in> (f g' \<Ztypecolon> T \<Rrightarrow> T))\<close>
 
+declare [[
+  \<phi>reason_default_pattern \<open>\<phi>Index_getter ?idx ?T _ _\<close> \<Rightarrow> \<open>\<phi>Index_getter ?idx ?T _ _\<close> (100),
+  \<phi>reason_default_pattern \<open>\<phi>Index_mapper ?idx ?T _ _\<close> \<Rightarrow> \<open>\<phi>Index_mapper ?idx ?T _ _\<close> (100)
+]]
+
+declare [[\<phi>trace_reasoning = 1]]
 
 lemma idx_step_value_V_tup_suc:
   \<open>idx_step_value (Suc i) (V_tup.mk (va # vs)) = idx_step_value i (V_tup.mk vs)\<close>
@@ -302,11 +259,11 @@ lemma idx_step_mod_value_V_tup_suc:
   by (metis NO_MATCH_I V_tup_mult_cons idx_step_mod_value_tup list_update_code(3) nth_Cons_Suc)
 
 
-lemma \<phi>Index_getter_tup_suc:
+lemma [\<phi>reason 1200]:
   \<open> \<phi>Index_getter (i # idx) X Y f
-\<Longrightarrow> \<phi>Index_getter (Suc i # idx) (\<clubsuit> T \<^emph> \<phi>Is_Tuple X) Y (f o snd)\<close>
+\<Longrightarrow> \<phi>Index_getter (Suc i # idx) (\<clubsuit> T \<^emph> X) Y (f o snd)\<close>
   unfolding \<phi>Index_getter_def
-  by (clarsimp simp add: \<phi>expns V_tup_mult idx_step_value_V_tup_suc)
+  apply (clarsimp simp add: \<phi>expns V_tup_mult idx_step_value_V_tup_suc)
 
 lemma \<phi>Index_getter_tup_0:
   \<open> \<phi>Index_getter idx X Y f
@@ -336,7 +293,6 @@ lemma \<phi>Index_mapper_tup_suc:
   apply (clarsimp simp add: \<phi>expns V_tup_mult idx_step_mod_value_V_tup_suc)
   by (metis V_tup_sep_disj idx_step_mod_value_tup)
 
-
 lemma \<phi>Index_mapper_tup_0:
   \<open> \<phi>Index_mapper idx X Y f
 \<Longrightarrow> \<phi>Index_mapper (0 # idx) (\<clubsuit> X) Y f\<close>
@@ -357,6 +313,39 @@ lemma \<phi>Index_mapper_arr:
   unfolding \<phi>Index_mapper_def Premise_def
   apply (clarsimp simp add: \<phi>expns V_tup_mult idx_step_mod_value_arr list_all2_conv_all_nth)
   by (metis nth_list_update)
+
+
+
+
+
+definition op_get_tuple :: "index list \<Rightarrow> TY \<Rightarrow> (VAL, VAL) proc'"
+  where "op_get_tuple idx T = (\<lambda>v.
+    \<phi>M_getV T id v (\<lambda>v'.
+    \<phi>M_assert (valid_index T idx) \<ggreater>
+    Return (\<phi>arg (index_value idx v'))
+))"
+
+term \<open>3-4-5\<close>
+
+definition op_set_tuple :: "index \<Rightarrow> TY \<Rightarrow> (VAL, VAL) proc'"
+  where "op_set_tuple idx T = (\<lambda>v.
+    \<phi>M_getV T V_tup.dest v (\<lambda>vals.
+    Return (\<phi>arg (vals ! idx))
+))"
+
+
+
+definition op_get_tuple :: "index list \<Rightarrow> TY \<Rightarrow> VAL proc"
+  where "op_get_tuple idx T = (\<lambda>(v#vs,res).
+    if valid_index T idx \<and> v \<in> Well_Type T
+    then Success (index_value idx v # vs, res)
+    else Fail)"
+
+
+term V_tup.mk
+
+
+
 
 
 end
