Phi_Semantics/PhiSem_Aggregate_Tuple.thy
@@ -1,0 +1,16 @@
+theory PhiSem_Aggregate_Tuple
+  imports PhiSem_Aggregate_Base
+begin
+
+section \<open>Semantics\<close>
+
+subsection \<open>Models\<close>
+
+subsubsection \<open>Type\<close>
+
+virtual_datatype tuple_ty = \<phi>empty_ty +
+  tup     :: \<open>'self list\<close>
+  array   :: \<open>'self \<times> nat\<close>
+
+
+end
